\documentclass{article}

\usepackage{amsmath}
\usepackage{amssymb}
\usepackage{textcmds}
\usepackage{graphicx}
\usepackage{subcaption}
\usepackage{float}
\usepackage{hhline}

\title{MAA202: Analysis\\Homework I}

\date{4$^{th}$ November 2019}
\author{Ma\"elys Solal\\Alexandre Hirsch\\Andr\'e Renom}

\begin{document}


	\pagenumbering{gobble}
	\maketitle

	\tableofcontents
	%\listoffigures
	\newpage
	\pagenumbering{arabic}
	\renewcommand{\thesubsubsection}{\thesubsection.\alph{subsubsection}}
	%\renewcommand{\thesection}{\Roman{section}} %To set Section numbering to Roman

\section{Exercise 1}
\subsection{} %Exercise 1.1

Let $B = \bar{B}(0,1) = \{x \in E \ | \ ||x|| \leq 1\}$ be the closed unit ball for the norm $||\cdot||$. Let us show that $B$ is cool. \\

Let us prove that $B$ is convex. \\
Take $x, y \in B$ and $t \in [0, 1]$. We want to prove that $tx + (1-t)y \in B$. To do so, we prove that $||tx + (1-t)y|| \leq 1$. 
\begin{align*}
 	||tx + (1-t)y|| &\leq ||tx|| + ||(1-t)y|| \quad \text{by the triangle inequality} \\
	&= |t|\cdot ||x|| + |1-t|\cdot ||y|| \quad \text{by homogeneity} \\
	&\leq t + (1-t) \quad \text{as} \  ||x|| \leq 1 \  \text{and} \  ||y|| \leq 1 \\
	&= 1 
\end{align*}
Which finally proves that B is convex. \\

We now prove that $B$ is bounded. \\
Take $x \in B$ then $||x|| \leq 1$ by definition of $B$. This proves that $B$ is bounded by $1$. \\

We now prove that $B$ is symmetric with respect to $0$. \\
Take $x \in B$ then $||x|| \leq 1$ by definition of $B$ and thus $|-1|\cdot||x|| \leq 1$ and by homogeneity $||-x|| \leq 1$ which proves $-x \in B$. \\
We have therefore proved that $B$ is symmetric with respect to $0$. \\

We finally prove that $0 \in \mathring{B}$ \\
Let $\widetilde{B}=B(0,1) = \{x \ | \  ||x|| < 1 \}$ be the open unit ball. We know $\widetilde{B} \subset B$ and $\widetilde{B}$ is open. As $\mathring{B}$ is the union of all open sets of $B$, we get $\widetilde{B} \subset \mathring{B}$. \\
By definition, $0 \in \widetilde{B}$ and hence $0 \in \mathring{B}$. 

\noindent Finally, we have proved that $B$ is cool.





\subsection{}%Exercise 1.2
We want to show that for a cool set $X$, and $\alpha,\beta \geq 0, \, \alpha X + \beta X = (\alpha + \beta )X$\\
We will procede by double inculsion, let us therefore first show that $\alpha X + \beta X \subseteq (\alpha + \beta )X$. We will take $a,b \in X$. Then $a\alpha + b\beta \in  \alpha X + \beta X$.
\begin{align*}
	a\alpha + b\beta = (\alpha + \beta )\left( \frac{\alpha}{\alpha + \beta}a +  \frac{\beta}{\alpha + \beta}b \right)
\end{align*}
We define $t := \frac{\alpha}{\alpha + \beta} \in [0,1]$, and thus $\frac{\beta}{\alpha + \beta} = t-1$. We therefore have:
\begin{align*}
	a\alpha + b\beta = (\alpha + \beta )\big(at + b(t-1)\big)
\end{align*}
By the definition of a cool set, we have that $X$ is convex, and hence for $a,b \in X$, we have $c:=ta + (t-1)b \in X$. Therefore:
\begin{align*}
	a\alpha + b\beta = (\alpha + \beta )c \in (\alpha + \beta )X
\end{align*}
We therefore have that $\alpha X + \beta X \subseteq (\alpha + \beta )X$.\\We now want to show that $\alpha X + \beta X \supseteq (\alpha + \beta )X$.\\ We take $x \in (\alpha + \beta )X$. Then there exists $y \in X$ such that:
\begin{align*}
	x &= (\alpha + \beta )y\\
	&= \alpha y + \beta y \in \alpha X + \beta X
\end{align*}
We therefore have that $\alpha X + \beta X \supseteq (\alpha + \beta )X$.\\ This concludes the proof that $\alpha X + \beta X = (\alpha + \beta )X$.




\subsection{}%Exercise 1.3
\subsubsection{}%Exercise 1.3.a

We want to show that for each $x \in E$, the set $N := \{a\,|\, x \in \alpha X\}$ is not empty. We start from the fact that $0 \in \mathring{X}$. Therefore it must also be true that there exists an $r > 0$ such that $B(0,r) \subset X$. We will define $\alpha := \frac{2||x||}{r}$. We know that $B(0,\alpha r) \subset \alpha X$. Since $B(0, \alpha r) = B(0, 2||x||)$, we have that $x \in \alpha X$, and hence $\alpha \in N$.

\subsubsection{}%Exercise 1.3.b

We want to show that $N_X(\lambda x) = |\lambda|N_X(x)$, we start from:
\begin{align*}
	N_X(\lambda x) &= \inf\{|\alpha | \, | \lambda x \in \alpha X\}
\end{align*}
But we know that $\lambda x \in \alpha X \Leftrightarrow \lambda x \in -\alpha X$, hence we can write:
\begin{align*}
	N_X(\lambda x) &= \inf\{|\alpha | \, | |\lambda| x \in \alpha X\}\\
	&= \inf\{|\lambda \alpha | \, | x \in \alpha X\}\\
	&= |\lambda|\inf\{|\alpha | \, | x \in \alpha X\}\\
	&= |\lambda|N_X(x)
\end{align*}
This concludes the proof.
\subsubsection{}%Exercise 1.3.c
We want to show that $N_X(x) = 0 \Rightarrow x=0$, we start from:
\begin{align*}
	N_X(0) &= \inf\{|\alpha | \, | \lambda x \in \alpha X\} = 0\\
	&\Rightarrow x \in 0 \times X\\
	&\Rightarrow ||x|| \leq 0 \times M_X\\
	&\Rightarrow x = 0
\end{align*}
This concludes the proof.


\subsubsection{}%Exercise 1.3.d

We want to show that the triangular inequality is true for $N_X$.\\ 
We therefore take $x,y \in E$.
\begin{align*}
N_X(x+y) &= \inf\{|\alpha| \ | \ (x+y) \in \alpha X\}\\
&= \inf\left\{|\alpha| \ | \ (x+y) \in \frac{\alpha}{2} X+ \frac{\alpha}{2} X\right\}\\
&= \inf\left\{|\alpha| \ | \ x \in \frac{\alpha}{2}  X\right\} +  \textrm{inf}\left\{|\alpha| \ | \ y\in \frac{\alpha}{2}  X\right\}\\
&\leq \inf\{|\alpha| \ | \ x\in \alpha X\} + \textrm{inf}\{|\alpha| \ | \ y\in \alpha X\}\\
&= N_X(x) + N_X(y)
\end{align*}
This concludes the proof that the triangular inequality holds for $N_X$, and by extension, that $N_X$ is a norm.

\subsection{} %Exercise 1.4

\subsubsection{} %Exercise 1.4.a

We want to show that $||x|| \leq MN_X(x) \quad \forall x \in E$. In order to do this, we start from the fact that $X$ is bounded by $M$ and that therefore $X \subset \bar{B}(0,M)$. We have from this that $x \in N_X(x)\bar{X} \subset N_X\bar{B}(0,M)$. Since $x \in N_X\bar{B}(0,M)$ then $||x|| \leq MN_X$. This concludes the proof that $|| \cdot ||$ is weaker than $N_x$.

\subsubsection{} %Exercise 1.4.b

We want to show that there exists an $\alpha$ such that for all $x$, $N_X(x) \leq \alpha ||x||$.
Since $0 \in \mathring{X}$, we can consider $r := sup\{r \, | \, B(0,r) \subset X \}$ with $r \neq 0$. We then have that for all $x$, $N_XB(0,r) \subset B(0,x)$. We therefore have that:
\begin{align*}
	N_Xr &\leq ||x||\\
	N_X &\leq \frac{1}{r}||x||
\end{align*}
This concludes the proof that $N_X$ is weaker than $|| \cdot ||$, and therefore also that they are equivalent.

\subsection{} %Exercise 1.5

We know that $x \in \bar{X}$ is equivalent to





 
%%% Table Format %%%

%\begin{figure}[H]
%\begin{tabular}{ |p{2cm}||p{1.7cm}||p{3.8cm}||p{3.1cm}|}
%\hline
%\multicolumn{4}{|c|}{Table of Results with Uncertainties} \\
%\hline
%Distance (m) & Time (ns) & Uncertainty (Distance) & Uncertainty (time) \\
%\hline
%\hline
%\end{tabular}
%\caption{Experimental Results Table With Uncertainties}
%\end{figure}


%%% Image Format %%%

%\begin{figure}[H]
%	\centering
%	\includegraphics[width=0.5\linewidth]{circuit.png}
%	\caption{Experiment 1: Circuit Set-Up}
%\end{figure}

%%% Equation Format %%%

%\begin{align*}
%	a &= 10
%	bcde &= 1
%\end{align*}


\end{document}